src/tls/Old.Handshake.fst
@@ -11,8 +11,6 @@ open TLSError
 open TLSInfo
 open TLSConstants
 open Range
-open HandshakeMessages // for the message syntax
-open HandshakeLog // for Outgoing
 open Old.Epochs
 
 module U32 = FStar.UInt32
@@ -23,8 +21,11 @@ module HST = FStar.HyperStack.ST
 module Epochs = Old.Epochs
 module KeySchedule = Old.KeySchedule
 module HMAC_UFCMA = Old.HMAC.UFCMA
+module HSM = HandshakeMessages
+module HSL = HandshakeLog
+module CH = Parsers.ClientHello
+module SH = Parsers.ServerHello
 // For readabililty, we try to open/abbreviate fewer modules
-
 
 (* A flag for runtime debugging of Handshake data.
    The F* normalizer will erase debug prints at extraction
@@ -62,7 +63,7 @@ type machineState =
   | C_Wait_Finished1           // TLS 1.3
   | C_Sent_EOED:
     digest ->
-    option HandshakeMessages.cr13 ->
+    option HSM.certificateRequest13 ->
     i:finishedId & cfk:KeySchedule.fink i -> machineState // TLS 1.3#20 aggravation
   | C_Wait_CCS1 of digest      // TLS resume, digest to be MACed by server
   | C_Wait_R_Finished1 of digest // TLS resume, digest to be MACed by server
@@ -295,11 +296,15 @@ let verify_binder hs (bkey:(i:binderId & bk:KeySchedule.binderKey i)) (tag:btag 
 // may be called both by client_ClientHello and client_HelloRetryRequest
 let client_Binders hs offer =
   match Nego.resume hs.nego with
-  | _, [] -> () // No PSK, no binders
-  | _, pskl -> // Nego may filter the PSKs
+  | _, [] ->
+    HandshakeLog.send hs.log (HSL.Msg (HSM.M_client_hello offer))
+  | _, pskl ->
     let binderKeys = KeySchedule.ks_client_13_get_binder_keys hs.ks pskl in
+    let blen = Extensions.bindersLen offer.CH.extensions in    
+    HSL.send_truncated hs.log (HSL.Msg (HSM.M_client_hello offer)) blen;
     let binders = map_ST2 hs compute_binder binderKeys in
-    HandshakeLog.send hs.log (Binders binders);
+    let bb = Parsers.OfferedPsks_binders.offeredPsks_binders_serializer32 binders in
+    HSL.send_raw hs.log bb;
 
     // Nego ensures that EDI is not sent in a 2nd ClientHello
     if Nego.find_early_data offer then
@@ -317,19 +322,19 @@ let client_Binders hs offer =
 val client_ClientHello: s:hs -> i:id -> ST (result unit) // (result (HandshakeLog.outgoing i))
   (requires fun h0 ->
     let n = HS.sel h0 Nego.(s.nego.state) in
-    let t = transcript h0 s.log in
+    let t = HSL.transcript h0 s.log in
     let k = HS.sel h0 s.ks.KeySchedule.state in
     match n with
     | Nego.C_Init nonce -> k = KeySchedule.(C (C_Init nonce)) /\ t = []
     | _ -> False )
   (ensures fun h0 r h1 ->
     let n = HS.sel h0 Nego.(s.nego.state) in
-    let t = transcript h0 s.log in
+    let t = HSL.transcript h0 s.log in
     let k = HS.sel h1 s.ks.KeySchedule.state in
     ( Correct? r ==>
       ( match n with
         | Nego.C_Offer offer -> (
-          ( if offer.ch_protocol_version = TLS_1p3
+          ( if offer.CH.version = TLS_1p3
             then
              k = KeySchedule.(C(C_13_wait_SH
               (nonce s)
@@ -339,8 +344,8 @@ val client_ClientHello: s:hs -> i:id -> ST (result unit) // (result (HandshakeLo
                  // + check that that the group and CommonDH.pubshare g gx match
               //(Nego.gs_of offer)
              ))
-            else k = KeySchedule.(C(C_12_Full_CH offer.ch_client_random)) /\
-          t = [ClientHello offer] ))
+            else k = KeySchedule.(C(C_12_Full_CH offer.CH.random)) /\
+          t = [HSL.Msg (HSM.M_client_hello offer)] ))
         | _ -> False )))
 
 let client_ClientHello hs i =
@@ -365,17 +370,18 @@ let client_ClientHello hs i =
   match Nego.client_ClientHello hs.nego shares with
   | Error z -> Error z
   | Correct offer ->
-    trace ("Binders length: "^string_of_int (FStar.UInt32.v (Extensions.bindersLen offer.ch_extensions)));
-    HandshakeLog.send hs.log (ClientHello offer);
     // Comptue and send PSK binders & 0-RTT signals
     client_Binders hs offer;
     // we may still need to keep parts of ch
     hs.state := C_Wait_ServerHello;
     Correct ()
 
+type hrr = unit
+
 let client_HelloRetryRequest (hs:hs) (hrr:hrr) : St incoming =
   trace "client_HelloRetryRequest";
-  let s = match Nego.group_of_hrr hrr with
+  let s =
+    match Nego.group_of_hrr hrr with
     | None ->
       // this case should only ever happen in QUIC stateless retry address validation
       trace "Server did not specify a group in HRR, re-using the previous choice"; None
@@ -387,7 +393,7 @@ let client_HelloRetryRequest (hs:hs) (hrr:hrr) : St incoming =
   match Nego.client_HelloRetryRequest hs.nego hrr s with
   | Error z -> InError z
   | Correct(ch) ->
-    HandshakeLog.send hs.log (ClientHello ch);
+    HSL.send hs.log (HSL.Msg (HSM.M_client_hello ch));
     client_Binders hs ch;
     // Note: we stay in Wait_ServerHello
     // Only the Nego state machine was moved by HRR
@@ -395,7 +401,7 @@ let client_HelloRetryRequest (hs:hs) (hrr:hrr) : St incoming =
 
 // requires !hs.state = Wait_ServerHello
 // ensures TLS 1.3 ==> installed handshake keys
-let client_ServerHello (s:hs) (sh:sh) (* digest:Hashing.anyTag *) : St incoming =
+let client_ServerHello (s:hs) (sh:HSM.serverHello) (* digest:Hashing.anyTag *) : St incoming =
   trace "client_ServerHello";
   match Nego.client_ServerHello s.nego sh with
   | Error z -> InError z
@@ -439,7 +445,7 @@ let client_ServerHello (s:hs) (sh:sh) (* digest:Hashing.anyTag *) : St incoming 
     | _ ->
       begin
         trace "Running classic TLS";
-        trace ("Offered SID="^(print_bytes mode.Nego.n_offer.ch_sessionID)^" Server SID="^(print_bytes mode.Nego.n_sessionID));
+        trace ("Offered SID="^(print_bytes mode.Nego.n_offer.CH.session_id)^" Server SID="^(print_bytes mode.Nego.n_sessionID));
         if Nego.resume_12 mode then
          begin // 1.2 resumption
           trace "Server accepted our 1.2 ticket.";
@@ -468,23 +474,36 @@ let client_ServerHello (s:hs) (sh:sh) (* digest:Hashing.anyTag *) : St incoming 
 (* receive Certificate...ServerHelloDone, with optional cert request. Not for TLS 1.3 *)
 val client_ServerHelloDone:
   hs ->
-  HandshakeMessages.crt ->
-  HandshakeMessages.ske ->
-  option HandshakeMessages.cr ->
+  HSM.certificate12 ->
+  ske_bytes: bytes -> //  HSM.serverKeyExchange
+  option HSM.certificateRequest12 ->
   ST incoming
   (requires (fun h -> True))
   (ensures (fun h0 i h1 -> True))
-let client_ServerHelloDone hs c ske ocr =
+
+let convert_kex = function
+  | Kex_RSA -> Correct HSM.Rsa
+  | Kex_DHE -> Correct HSM.Dhe
+  | Kex_ECDHE -> Correct HSM.Ecdhe
+  | _ -> fatal Internal_error "Incorrect key exchange selected for 1.2"
+
+let client_ServerHelloDone hs c ske_bytes ocr =
     trace "processing ...ServerHelloDone";
-    match Nego.client_ServerKeyExchange hs.nego c ske ocr with
+    let kex = Nego.kexAlg (Nego.getMode hs.nego) in
+    match convert_kex kex with
+    | Error z -> InError z
+    | Correct kex ->
+    match HSM.serverKeyExchange_parser32 kex ske_bytes with
+    | None -> InError (fatalAlert Decode_error, "invalid client key exchange")
+    | Some (ske, _) ->
+    match Nego.client_ServerKeyExchange hs.nego c kex ske ocr with
     | Error z -> InError z
     | Correct mode -> (
-      ( match ocr with
-        | None -> ()
-        | Some cr ->
-            trace "processing certificate request (TODO)";
-            let cc = {crt_chain = []} in
-            HandshakeLog.send hs.log (Certificate cc));
+      (match ocr with
+      | None -> ()
+      | Some cr ->
+        trace "processing certificate request (TODO)";
+        HandshakeLog.send hs.log (HSL.Msg12 (HSM.M12_certificate [])));
 
       let gy = Some?.v (mode.Nego.n_server_share) in // already set in KS
       let gx =
@@ -495,9 +514,13 @@ let client_ServerHelloDone hs c ske ocr =
         (Nego.emsFlag mode) // a flag controlling the use of ems
         gy in
       let (|g, _|) = gy in
-      let msg = ClientKeyExchange ({cke_kex_c = kex_c_of_dh_key #g gx}) in
+      let msg = HSM.M12_client_key_exchange (
+        match kex with
+	| HSM.Ecdhe -> CommonDH.serialize_raw gx
+	| HSM.Dhe -> CommonDH.serialize_raw gx
+	| _ -> magic()) in
       let ha = verifyDataHashAlg_of_ciphersuite (mode.Nego.n_cipher_suite) in
-      let digestClientKeyExchange = HandshakeLog.send_tag #ha hs.log msg  in
+      let digestClientKeyExchange = HandshakeLog.send_tag #ha hs.log (HSL.Msg12 msg)  in
       let cfin_key, app_keys = KeySchedule.ks_client_12_set_session_hash hs.ks digestClientKeyExchange in
       register hs app_keys;
       // we send CCS then Finished;  we will use the new keys only after CCS
@@ -505,22 +528,27 @@ let client_ServerHelloDone hs c ske ocr =
       trace ("digest is "^print_bytes digestClientKeyExchange);
       //let cvd = TLSPRF.verifyData (mode.Nego.n_protocol_version,mode.Nego.n_cipher_suite) cfin_key Client digestClientKeyExchange in
       let cvd = TLSPRF.finished12 ha cfin_key Client digestClientKeyExchange in
-      let digestClientFinished = HandshakeLog.send_CCS_tag #ha hs.log (Finished ({fin_vd = cvd})) false in
+      let fin = HSM.M12_finished cvd in
+      let digestClientFinished = HandshakeLog.send_CCS_tag #ha hs.log (HSL.Msg12 fin) false in
       hs.state := C_Wait_CCS2 digestClientFinished;
       InAck false false)
 
 #set-options "--admit_smt_queries true"
-private val client_ClientFinished_13: hs -> digest -> option HandshakeMessages.cr13 -> (i:finishedId & cfk:KeySchedule.fink i) -> St unit
+private val client_ClientFinished_13: hs -> digest -> option HSM.certificateRequest13 -> (i:finishedId & cfk:KeySchedule.fink i) -> St unit
+
 let client_ClientFinished_13 hs digestServerFinished ocr cfin_key =
   let mode = Nego.getMode hs.nego in
   let ha = verifyDataHashAlg_of_ciphersuite (mode.Nego.n_cipher_suite) in
   let digest =
     match ocr with
-    | Some cr -> HandshakeLog.send_tag #ha hs.log (Certificate13 ({crt_request_context = empty_bytes; crt_chain13 = []}))
+    | Some cr ->
+      let open Parsers.Certificate13 in
+      let c = ({certificate_request_context = empty_bytes; certificate_list = []}) in
+      HandshakeLog.send_tag #ha hs.log (HSL.Msg13 (HSM.M13_certificate c))
     | None -> digestServerFinished in
   let (| finId, cfin_key |) = cfin_key in
   let cvd = HMAC_UFCMA.mac cfin_key digest in
-  let digest_CF = HandshakeLog.send_tag #ha hs.log (Finished ({fin_vd = cvd})) in
+  let digest_CF = HandshakeLog.send_tag #ha hs.log (HSL.Msg13 (HSM.M13_finished cvd)) in
   KeySchedule.ks_client_13_cf hs.ks digest_CF; // For Post-HS
   Epochs.incr_reader hs.epochs; // to ATK
   HandshakeLog.send_signals hs.log (Some (true, false)) true; //was: Epochs.incr_writer hs.epochs
@@ -529,50 +557,53 @@ let client_ClientFinished_13 hs digestServerFinished ocr cfin_key =
 (* receive EncryptedExtension...ServerFinished for TLS 1.3, roughly mirroring client_ServerHelloDone *)
 val client_ServerFinished_13:
   s: hs ->
-  ee: HandshakeMessages.ee ->
-  ocr: option HandshakeMessages.cr13 ->
-  oc: option HandshakeMessages.crt13 ->
-  ocv: option HandshakeMessages.cv ->
+  ee: HSM.encryptedExtensions ->
+  ocr: option HSM.certificateRequest13 ->
+  oc: option HSM.certificate13 ->
+  ocv: option HSM.certificateVerify13 ->
   svd: bytes ->
   digestCert: option Hashing.anyTag ->
   digestCertVerify: Hashing.anyTag ->
   digestServerFinished: Hashing.anyTag ->
   St incoming
-let client_ServerFinished_13 hs ee ocr oc ocv (svd:bytes) digestCert digestCertVerify digestServerFinished =
-    let oc = match oc with | None -> None | Some c -> Some c.crt_chain13 in
-    let cfg = Nego.local_config hs.nego in
-    match Nego.clientComplete_13 hs.nego ee ocr oc ocv digestCert with
-    | Error z -> InError z
-    | Correct mode ->
-        // ADL: 4th returned value is the exporter master secret.
-        // should be passed to application somehow --- store in Nego? We need agreement.
-        let (sfin_key, cfin_key, app_keys, exporter_master_secret) = KeySchedule.ks_client_13_sf hs.ks digestServerFinished in
-        let (| finId, sfin_key |) = sfin_key in
-        if not (HMAC_UFCMA.verify sfin_key digestCertVerify svd)
-        then InError (fatalAlert Decode_error, "Finished MAC did not verify: expected digest "^print_bytes digestCertVerify )
-        else
-	 begin
-          export hs exporter_master_secret;
-          register hs app_keys; // ATKs are ready to use in both directions
 
-          // EOED emitting (not used for QUIC)
-          if Nego.zeroRTT mode && not cfg.is_quic then
-	   begin
-            trace "Early data accepted; emitting EOED.";
-            let ha = Nego.hashAlg mode in
-            let digestEOED = HandshakeLog.send_tag #ha hs.log EndOfEarlyData in
-            HandshakeLog.send_signals hs.log (Some (false, false)) false;
-            hs.state := C_Sent_EOED digestEOED ocr cfin_key;
-            InAck false false
-	   end
-          else
-	   begin
-            (if Nego.zeroRTT mode then trace "Early data accepted (QUIC, no EOED)."
-	    else trace "Early data rejected");
-            client_ClientFinished_13 hs digestServerFinished ocr cfin_key;
-            InAck true false // Client 1.3 ATK; next the client will read again to send Finished, writer++, and the Complete signal
-           end
-	 end // moving to C_Complete
+let client_ServerFinished_13 hs ee ocr oc ocv (svd:bytes) digestCert digestCertVerify digestServerFinished =
+  let oc =
+    let open Parsers.Certificate13 in
+    match oc with | None -> None | Some c -> Some c.certificate_list in
+  let cfg = Nego.local_config hs.nego in
+  match Nego.clientComplete_13 hs.nego ee ocr oc ocv digestCert with
+  | Error z -> InError z
+  | Correct mode ->
+    // ADL: 4th returned value is the exporter master secret.
+       // should be passed to application somehow --- store in Nego? We need agreement.
+       let (sfin_key, cfin_key, app_keys, exporter_master_secret) = KeySchedule.ks_client_13_sf hs.ks digestServerFinished in
+       let (| finId, sfin_key |) = sfin_key in
+       if not (HMAC_UFCMA.verify sfin_key digestCertVerify svd)
+       then InError (fatalAlert Decode_error, "Finished MAC did not verify: expected digest "^print_bytes digestCertVerify )
+       else
+       begin
+         export hs exporter_master_secret;
+         register hs app_keys; // ATKs are ready to use in both directions
+
+         // EOED emitting (not used for QUIC)
+         if Nego.zeroRTT mode && not cfg.is_quic then
+	 begin
+           trace "Early data accepted; emitting EOED.";
+           let ha = Nego.hashAlg mode in
+           let digestEOED = HandshakeLog.send_tag #ha hs.log (HSL.Msg13 (HSM.M13_end_of_early_data ())) in
+           HandshakeLog.send_signals hs.log (Some (false, false)) false;
+           hs.state := C_Sent_EOED digestEOED ocr cfin_key;
+           InAck false false
+	 end
+         else
+	 begin
+           (if Nego.zeroRTT mode then trace "Early data accepted (QUIC, no EOED)."
+	   else trace "Early data rejected");
+           client_ClientFinished_13 hs digestServerFinished ocr cfin_key;
+           InAck true false // Client 1.3 ATK; next the client will read again to send Finished, writer++, and the Complete signal
+         end
+       end // moving to C_Complete
 
 let rec iutf8 (m:bytes) : St (s:string{String.length s < pow2 30 /\ utf8_encode s = m}) =
     match iutf8_opt m with
@@ -581,21 +612,22 @@ let rec iutf8 (m:bytes) : St (s:string{String.length s < pow2 30 /\ utf8_encode 
 
 // Processing of the server CCS and optional NewSessionTicket
 // This is used both in full handshake and resumption
-let client_NewSessionTicket_12 (hs:hs) (resume:bool) (digest:Hashing.anyTag) (ost:option sticket)
+let client_NewSessionTicket_12 (hs:hs) (resume:bool) (digest:Hashing.anyTag) (ost:option HSM.newSessionTicket12)
   : St incoming =
+  let open Parsers.NewSessionTicket12 in
   trace (
     "Processing server CCS ("
     ^(if resume then "resumption" else "full handshake")^"). "
     ^(match ost with
      | None -> "No ticket sent."
-     | Some {sticket_ticket = t} -> "Ticket: "^(print_bytes t)));
+     | Some {ticket = t} -> "Ticket: "^(print_bytes t)));
   hs.state :=
     (if resume then C_Wait_R_Finished1 digest
     else C_Wait_Finished2 digest);
   Epochs.incr_reader hs.epochs;
   let mode = Nego.getMode hs.nego in
   match ost, Nego.sendticket_12 mode with
-  | Some {sticket_ticket = tid}, true ->
+  | Some {ticket = tid}, true ->
     let cfg = Nego.local_config hs.nego in
     let sni = iutf8 (Nego.get_sni mode.Nego.n_offer) in
     let (msId, ms) = KeySchedule.ks_12_ms hs.ks in
@@ -609,27 +641,30 @@ let client_NewSessionTicket_12 (hs:hs) (resume:bool) (digest:Hashing.anyTag) (os
   | None, true -> InError (fatalAlert Unexpected_message, "missing expected NewSessionTicket message")
 
 // Process an incoming ticket (1.3)
-let client_NewSessionTicket_13 (hs:hs) (st13:sticket13)
+let client_NewSessionTicket_13 (hs:hs) (st13:HSM.newSessionTicket13)
   : St incoming =
+  let open Parsers.NewSessionTicket13 in
   let open Parsers.NewSessionTicketExtension in
-  let tid = st13.ticket13_ticket in
-  trace ("Received ticket: "^(hex_of_bytes tid));
+  let tid = st13.ticket in
+  let nonce = st13.ticket_nonce in
+  let age_add = st13.ticket_age_add in
+  trace ("Received ticket: "^(hex_of_bytes tid)^" nonce: "^(hex_of_bytes nonce));
   let mode = Nego.getMode hs.nego in
   let CipherSuite13 ae h = mode.Nego.n_cipher_suite in
-  let t_ext = st13.ticket13_extensions in
+  let t_ext = st13.extensions in
   let ed = List.Tot.find NSTE_early_data? t_ext in
   let now = UInt32.uint_to_t (FStar.Date.secondsFromDawn()) in
-  let pskInfo = PSK.({
-    ticket_nonce = Some st13.ticket13_nonce;
+  let pskInfo = TLSConstants.({
+    ticket_nonce = Some nonce;
     time_created = now;
-    ticket_age_add = st13.ticket13_age_add;
+    ticket_age_add = age_add;
     allow_early_data = Some? ed;
     allow_dhe_resumption = true;
     allow_psk_resumption = true;
     early_ae = ae; early_hash = h;
     identities = (empty_bytes, empty_bytes); // TODO certs
   }) in
-  let psk = KeySchedule.ks_client_13_rms_psk hs.ks st13.ticket13_nonce in
+  let psk = KeySchedule.ks_client_13_rms_psk hs.ks nonce in
   let sni = iutf8 (Nego.get_sni mode.Nego.n_offer) in
   let cfg = Nego.local_config hs.nego in
   let valid_ed =
@@ -651,7 +686,7 @@ let client_ServerFinished hs f digestClientFinished =
   let ha = verifyDataHashAlg_of_ciphersuite mode.Nego.n_cipher_suite in
   let expected_svd = TLSPRF.finished12 ha sfin_key Server digestClientFinished in
   //let expected_svd = TLSPRF.verifyData (mode.Nego.n_protocol_version,mode.Nego.n_cipher_suite) sfin_key Server digestClientFinished in
-  if f.fin_vd = expected_svd
+  if f = expected_svd
   then (
     hs.state := C_Complete; // ADL: TODO need a proper renego state Idle (Some (vd,svd)))};
     InAck false true // Client 1.2 ATK
@@ -667,10 +702,10 @@ let client_R_ServerFinished hs f digestNewSessionTicket digestServerFinished
   let mode = Nego.getMode hs.nego in
   let ha = verifyDataHashAlg_of_ciphersuite mode.Nego.n_cipher_suite in
   let expected_svd = TLSPRF.finished12 ha sfin_key Server digestNewSessionTicket in
-  if f.fin_vd = expected_svd
+  if f = expected_svd
   then (
     let cvd = TLSPRF.finished12 ha sfin_key Client digestServerFinished in
-    let _ = HandshakeLog.send_CCS_tag #ha hs.log (Finished ({fin_vd = cvd})) true in
+    let _ = HandshakeLog.send_CCS_tag #ha hs.log (HSL.Msg12 (HSM.M12_finished cvd)) true in
     hs.state := C_Complete; // ADL: TODO need a proper renego state Idle (Some (vd,svd)))};
     InAck false false // send_CCS_tag buffers the complete
   )
@@ -682,6 +717,7 @@ let client_R_ServerFinished hs f digestNewSessionTicket digestServerFinished
 (* called by server_ClientHello after sending TLS 1.2 ServerHello *)
 // static precondition: n.n_protocol_version <> TLS_1p3 && Some? n.n_sigAlg && (n.n_kexAlg = Kex_DHE || n.n_kexAlg = Kex_ECDHE)
 // should instead use Nego for most of this processing
+
 val server_ServerHelloDone: hs -> St incoming // why do I need an explicit val?
 let server_ServerHelloDone hs =
   trace "Sending ...ServerHelloDone";
@@ -703,7 +739,6 @@ let server_ServerHelloDone hs =
     | Error z -> InError z
     | Correct signature ->
       begin
-      let ske = {ske_kex_s = kex_s; ske_signed_params = signature} in
       HandshakeLog.send hs.log (Certificate ({crt_chain = Cert.chain_down chain}));
       HandshakeLog.send hs.log (ServerKeyExchange ske);
       HandshakeLog.send hs.log ServerHelloDone;
